

1. From problem 14.13, we have for  $k \neq 0$

$$\left\langle \frac{dP_k}{d\Omega} \right\rangle = \frac{e^2 k^2 \omega_0^4}{(2\pi c)^3} \left| \int_0^T e^{ik\omega_0[t-\mathbf{n}\cdot\mathbf{x}(t)/c]} \mathbf{n} \times \mathbf{v} dt \right|^2 \quad (1)$$

Denoting  $b \equiv \sqrt{1-\epsilon^2}a$ , we have

$$\mathbf{x}(u) = a(\cos u - \epsilon)\hat{\mathbf{x}} + b \sin u \hat{\mathbf{y}} \quad (2)$$

$$(3)$$

It is most convenient to evaluate the integral in variable  $u$ . First, the phase factor can be simplified as

$$e^{ik\omega_0[t-\mathbf{n}\cdot\mathbf{x}(u)/c]} = \exp \left[ \overbrace{ik\omega_0 t - ik\left(\frac{\omega_0 a}{c}\right) \sin \theta \cos \phi (\cos u - \epsilon) - \left(\frac{\omega_0 b}{c}\right) \sin \theta \sin \phi \sin u}^{\text{ignored for nonrelativistic motion}} \right] \\ \approx e^{ik\omega_0 t} = e^{ik(u-\epsilon \sin u)} \quad (4)$$

Next, notice that

$$\mathbf{n} \times \mathbf{v} dt = \mathbf{n} \times \frac{d\mathbf{x}}{du} du = (\sin \theta \cos \phi \hat{\mathbf{x}} + \sin \theta \sin \phi \hat{\mathbf{y}} + \cos \theta \hat{\mathbf{z}}) \times (-a \sin u \hat{\mathbf{x}} + b \cos u \hat{\mathbf{y}}) du \\ = [-b \cos \theta \cos u \hat{\mathbf{x}} - a \cos \theta \sin u \hat{\mathbf{y}} + (a \sin \theta \sin \phi \sin u + b \sin \theta \cos \phi \cos u) \hat{\mathbf{z}}] du \quad (5)$$

turning the integral in (1) into

$$\int_0^T e^{ik\omega_0[t-\mathbf{n}\cdot\mathbf{x}(t)/c]} \mathbf{n} \times \mathbf{v} dt = \mathbf{I}_x + \mathbf{I}_y + \mathbf{I}_z \quad (6)$$

where

$$\mathbf{I}_x = -b \cos \theta \hat{\mathbf{x}} \int_0^{2\pi} e^{ik(u-\epsilon \sin u)} \cos u du \quad (7)$$

$$\mathbf{I}_y = -a \cos \theta \hat{\mathbf{y}} \int_0^{2\pi} e^{ik(u-\epsilon \sin u)} \sin u du \quad (8)$$

$$\mathbf{I}_z = \sin \theta \hat{\mathbf{z}} \left[ a \sin \phi \int_0^{2\pi} e^{ik(u-\epsilon \sin u)} \sin u du + b \cos \phi \int_0^{2\pi} e^{ik(u-\epsilon \sin u)} \cos u du \right] \quad (9)$$

With the Jacobi-Anger expansion

$$e^{iz \sin \phi} = \sum_{n=-\infty}^{\infty} J_n(z) e^{in\phi} \quad (10)$$

we can write

$$e^{-ike \sin u} = \sum_{n=-\infty}^{\infty} J_n(-k\epsilon) e^{inu} \quad J_n(-x) = (-1)^n J_n(x) \\ = \sum_{n=-\infty}^{\infty} (-1)^n J_n(k\epsilon) e^{inu} \quad (11)$$

The  $\cos u$  integral in (7) becomes

$$\int_0^{2\pi} e^{ik(u-\epsilon \sin u)} \cos u du = \sum_{n=-\infty}^{\infty} (-1)^n J_n(k\epsilon) \frac{1}{2} \int_0^{2\pi} \overbrace{[e^{i(k+n+1)u} + e^{i(k+n-1)u}]}^{2\pi(\delta_{k+n+1,0} + \delta_{k+n-1,0})} du \\ = \pi [(-1)^{k+1} J_{-(k+1)}(k\epsilon) + (-1)^{k-1} J_{-(k-1)}(k\epsilon)] \quad J_{-n}(x) = (-1)^n J_n(x) \\ = \pi [J_{k+1}(k\epsilon) + J_{k-1}(k\epsilon)] \quad J_{k-1}(x) + J_{k+1}(x) = \frac{2k}{x} J_k(x) \\ = \frac{2\pi}{\epsilon} J_k(k\epsilon) \quad (12)$$

The  $\sin u$  integral in (8) becomes

$$\begin{aligned} \int_0^{2\pi} e^{ik(u-\epsilon \sin u)} \sin u du &= \sum_{n=-\infty}^{\infty} (-1)^n J_n(k\epsilon) \frac{1}{2i} \int_0^{2\pi} \overbrace{[e^{i(k+n+1)u} - e^{i(k+n-1)u}]}^{2\pi(\delta_{k+n+1,0} - \delta_{k+n-1,0})} du \\ &= \frac{\pi}{i} [J_{k+1}(k\epsilon) - J_{k-1}(k\epsilon)] \quad J_{k-1}(x) - J_{k+1}(x) = 2J'_k(x) \\ &= 2\pi i J'_k(k\epsilon) \end{aligned} \quad (13)$$

Substituting (12) and (13) back into (7)–(9) gives

$$\mathbf{I}_x = -\frac{2\pi b \cos \theta}{\epsilon} J_k(k\epsilon) \hat{\mathbf{x}} \quad (14)$$

$$\mathbf{I}_y = -2\pi i a \cos \theta J'_k(k\epsilon) \hat{\mathbf{y}} \quad (15)$$

$$\mathbf{I}_z = 2\pi \sin \theta \left[ i a \sin \phi J'_k(k\epsilon) + \frac{b \cos \phi}{\epsilon} J_k(k\epsilon) \right] \hat{\mathbf{z}} \quad (16)$$

Thus

$$\begin{aligned} |\mathbf{I}|^2 &= 4\pi^2 \left\{ \frac{b^2 \cos^2 \theta}{\epsilon^2} J_k^2(k\epsilon) + a^2 \cos^2 \theta J_k'^2(k\epsilon) + \sin^2 \theta \left[ a^2 \sin^2 \phi J_k'^2(k\epsilon) + \frac{b^2 \cos^2 \phi}{\epsilon^2} J_k^2(k\epsilon) \right] \right\} \\ &= 4\pi^2 \left[ \frac{b^2}{\epsilon^2} (\cos^2 \theta + \sin^2 \theta \cos^2 \phi) J_k^2(k\epsilon) + a^2 (\cos^2 \theta + \sin^2 \theta \sin^2 \phi) J_k'^2(k\epsilon) \right] \end{aligned} \quad (17)$$

Recalling that  $b^2 = (1 - \epsilon^2) a^2$ , we can write

$$\left\langle \frac{dP_k}{d\Omega} \right\rangle = \frac{e^2 k^2 \omega_0^4 a^2}{2\pi c^3} \left[ \left( \frac{1 - \epsilon^2}{\epsilon^2} \right) (\cos^2 \theta + \sin^2 \theta \cos^2 \phi) J_k^2(k\epsilon) + (\cos^2 \theta + \sin^2 \theta \sin^2 \phi) J_k'^2(k\epsilon) \right] \quad (18)$$

With the solid angle integration

$$\int (\cos^2 \theta + \sin^2 \theta \cos^2 \phi) d\Omega = \int (\cos^2 \theta + \sin^2 \theta \sin^2 \phi) d\Omega = \frac{8\pi}{3} \quad (19)$$

we have the total power for the  $k$ th harmonic

$$P_k = \frac{4e^2 k^2 \omega_0^4 a^2}{3c^3} \left[ \left( \frac{1 - \epsilon^2}{\epsilon^2} \right) J_k^2(k\epsilon) + J_k'^2(k\epsilon) \right] \quad (20)$$

2. For circular orbit,  $\epsilon \rightarrow 0$ . Under this limit, all harmonics but  $k = 1$  vanishes, and for  $k = 1$ ,

$$\lim_{\epsilon \rightarrow 0} \left[ \left( \frac{1 - \epsilon^2}{\epsilon^2} \right) J_1^2(\epsilon) \right] = \lim_{\epsilon \rightarrow 0} \left[ \left( \frac{1 - \epsilon^2}{\epsilon^2} \right) \left( \frac{\epsilon}{2} \right)^2 \right] = \frac{1}{4} \quad \lim_{\epsilon \rightarrow 0} J_1'^2(\epsilon) = \frac{1}{4} \quad (21)$$

which gives

$$P_1 = \frac{2e^2 \omega_0^4 a^2}{3c^3} \quad (22)$$

agreeing with problem 14.21 (a) (under the approximation  $\gamma \rightarrow 1$ ).